ironfleet/src/Dafny/Distributed/Protocol/ZooKeeper/ZKEnvironment.dfy
@@ -17,7 +17,7 @@ type Config = seq<EndPoint>
 
 datatype ZKMessage = 
     | FollowerInfo(sid:nat, latestZxid:Zxid)
-    | LeaderInfo(sid:nat, serial:int, newZxid:Zxid)
+    | LeaderInfo(sid:nat, serial:nat, newZxid:Zxid)
     | AckEpoch(sid:nat, lastLoggedZxid:Zxid, lastAcceptedEpoch:int)
     | SyncDIFF(sid:nat, lastProcessedZxid:Zxid)
     | SyncSNAP(sid:nat, leaderDb: ZKDatabase, lastProcessedZxid:Zxid)
